Validate submission ce67ea8d-1f5d-4fc1-b46a-10268d2a94a9
Co-authored-by: terrapinelf <166810331+terrapinelf@users.noreply.github.com>

Challenge/Modexp/Submission/Proofs/Bytecode/Artifact.lean
@@ -1151,17 +1151,7 @@ def submissionInstructions : List Instr :=
  .op .AND,
  .op .MLOAD,
  .op .MULMOD,
- .op .JUMPDEST,
- .op .JUMPDEST,
- .op .JUMPDEST,
- .op .JUMPDEST,
- .op .JUMPDEST,
- .op .JUMPDEST,
- .op .JUMPDEST,
- .op .JUMPDEST,
- .op .JUMPDEST,
- .op .JUMPDEST,
- .push 6 100447932865371,
+ .push 16 121434099567864314412422772696005958491,
  .op .POP,
  .op (.Dup { idx := 1 }),
  .op (.Dup { idx := 0 }),
@@ -1569,16 +1559,7 @@ def submissionInstructions : List Instr :=
  .op .AND,
  .op .MLOAD,
  .op .MULMOD,
- .op .JUMPDEST,
- .op .JUMPDEST,
- .op .JUMPDEST,
- .op .JUMPDEST,
- .op .JUMPDEST,
- .op .JUMPDEST,
- .op .JUMPDEST,
- .op .JUMPDEST,
- .op .JUMPDEST,
- .push 7 25714670813535067,
+ .push 16 121434099567864314413212591480656059227,
  .op .POP,
  .op (.Dup { idx := 1 }),
  .op (.Dup { idx := 0 }),
@@ -4416,7 +4397,7 @@ def submissionInstructions : List Instr :=
  .push 0 0,
  .op .RETURN]
 
-theorem submissionInstructions_count : submissionInstructions.length = 4393 := by
+theorem submissionInstructions_count : submissionInstructions.length = 4374 := by
   decide
 
 theorem assemble_submissionInstructions :
